CTL/Equivalence.lean
@@ -3,75 +3,81 @@ import CTL.Basic
 import CTL.Satisfaction
 
 namespace CTL
-variable {p : Type}
-         {Φ Φ' Ψ Ψ' : @StateFormula p}
+variable {p α β : Type}
+         [αSat : StateSatisfiable p α]
+         [βSat : StateSatisfiable p β]
+         (Φ : α)
+         (Ψ : β)
 
 -- Sat(Φ) = Sat(Ψ)
 @[simp]
-def Equiv (Φ Ψ : @StateFormula p) :=
-  ∀{s a : Type} , ∀{ts : @TS s a p}, satStateSet ts Φ = satStateSet ts Ψ
+def Equiv :=
+  ∀{s a : Type} , ∀{ts : @TS s a p}, setOfSatStates ts Φ = setOfSatStates ts Ψ
 
 -- TS ⊨ Φ ↔ TS ⊨ Ψ
 @[simp]
-def Equiv' (Φ Ψ : @StateFormula p) :=
+def Equiv' :=
   ∀{s a : Type} , ∀{ts : @TS s a p}, Sat ts Φ ↔ Sat ts Ψ
 
 namespace Equiv
 @[simp]
-theorem equiv'_of_equiv : Equiv Φ Ψ → Equiv' Φ Ψ := by
+theorem equiv'_of_equiv : Equiv (p := p) Φ Ψ → Equiv' (p := p) Φ Ψ := by
   simp [Equiv, Equiv']
   intro h _ _ _
   rewrite [h]
   trivial
 
-instance : IsRefl (@StateFormula p) Equiv where
+instance : IsRefl α (Equiv (p := p)) where
   refl := by simp
 
-instance : IsSymm (@StateFormula p) Equiv where
+instance : IsSymm α (Equiv (p := p)) where
   symm := fun Φ Ψ => by simp; intros h _ _ _; exact Eq.symm h
 
-instance : IsTrans (@StateFormula p) Equiv where
+instance : IsTrans α (Equiv (p := p)) where
   trans := fun _ _ _ h₁ h₂ => Trans.trans h₁ h₂
 
-instance : IsPreorder (@StateFormula p) Equiv where
+instance : IsPreorder α (Equiv (p := p)) where
 
-instance : IsEquiv (@StateFormula p) Equiv where
+instance : IsEquiv α (Equiv (p := p)) where
+
+namespace StateFormula
+variable {Φ Φ' Φ₁ Φ₁' Φ₂ Φ₂' Ψ Ψ' : @StateFormula p}
 
 @[simp]
-theorem conj_congr (h₁ : Equiv Φ₁ Φ₁') (h₂ : Equiv Φ₂ Φ₂') : Equiv (Φ₁ ⬝∧ Φ₂) (Φ₁' ⬝∧ Φ₂') := by
-  simp [Equiv, satStateSet, SatState, StateSat, Set.ext_iff] at *
+theorem conj_congr (h₁ : Equiv (p := p) Φ₁ Φ₁') (h₂ : Equiv (p := p) Φ₂ Φ₂') : Equiv (p := p) (Φ₁ ⬝∧ Φ₂) (Φ₁' ⬝∧ Φ₂') := by
+  simp [Equiv, setOfSatStates, SatState, StateSatisfiable.StateSat, Set.ext_iff] at *
   intros _ _ _ _
   constructor
   . rintro ⟨sat₁, sat₂⟩; constructor; exact (h₁ _).1 sat₁; exact (h₂ _).1 sat₂
   . rintro ⟨sat₁, sat₂⟩; constructor; exact (h₁ _).2 sat₁; exact (h₂ _).2 sat₂
 
 @[simp]
-theorem neg_congr (h : Equiv Φ Φ') : Equiv (⬝¬Φ) (⬝¬Φ') := by
-  simp [Equiv, satStateSet, SatState, StateSat, Set.ext_iff] at *
+theorem neg_congr (h : Equiv (p := p) Φ Φ') : Equiv (p := p) (⬝¬Φ) (⬝¬Φ') := by
+  simp [Equiv, setOfSatStates, SatState, StateSatisfiable.StateSat, Set.ext_iff] at *
   intros _ _ _ _
   constructor
   . rintro negSat sat; exact negSat ((h _).2 sat)
   . rintro negSat sat; exact negSat ((h _).1 sat)
 
 @[simp]
-theorem exist_next_congr (h : Equiv Φ Φ') : Equiv (⬝∃⬝◯Φ) (⬝∃⬝◯Φ') := by
-  simp [Equiv, satStateSet, SatState, StateSat, PathSat, Set.ext_iff] at *
+theorem exist_next_congr (h : Equiv (p := p) Φ Φ') : Equiv (p := p) (⬝∃⬝◯Φ) (⬝∃⬝◯Φ') := by
+  simp [Equiv, setOfSatStates, SatState, StateSatisfiable.StateSat, Set.ext_iff] at *
   intros _ _ _ _
   constructor
   . rintro ⟨π, sat⟩; exact ⟨π, (h _).1 sat⟩
   . rintro ⟨π, sat⟩; exact ⟨π, (h _).2 sat⟩
 
 @[simp]
-theorem exist_untl_congr (h₁ : Equiv Φ Φ') (h₂ : Equiv Ψ Ψ') : Equiv (⬝∃(Φ ⬝U Ψ)) (⬝∃(Φ' ⬝U Ψ')) := by
-  simp [Equiv, satStateSet, SatState, StateSat, PathSat, Set.ext_iff] at *
+theorem exist_untl_congr (h₁ : Equiv (p := p) Φ Φ') (h₂ : Equiv (p := p) Ψ Ψ') : Equiv (p := p) (⬝∃(Φ ⬝U Ψ)) (⬝∃(Φ' ⬝U Ψ')) := by
+  simp [Equiv, setOfSatStates, SatState, StateSatisfiable.StateSat, Set.ext_iff] at *
   intros _ _ _ _
   constructor
   . rintro ⟨π, j, ⟨satJ, satK⟩⟩; exact ⟨π, j, ⟨(h₂ _).1 satJ, fun k => (h₁ _).1 (satK k)⟩⟩
   . rintro ⟨π, j, ⟨satJ, satK⟩⟩; exact ⟨π, j, ⟨(h₂ _).2 satJ, fun k => (h₁ _).2 (satK k)⟩⟩
 
 @[simp]
-theorem all_next_congr (h : Equiv Φ Φ') : Equiv (⬝∀⬝◯Φ) (⬝∀⬝◯Φ') := by
-  simp [Equiv, satStateSet, SatState, StateSat, PathSat, Set.ext_iff] at *
+theorem all_next_congr (h : Equiv (p := p) Φ Φ') : Equiv (p := p) (⬝∀⬝◯Φ) (⬝∀⬝◯Φ') := by
+  simp [Equiv, setOfSatStates, SatState, StateSatisfiable.StateSat, Set.ext_iff] at *
   intros _ _ _ _
   constructor
   . rintro sat π; rw [← h]; exact sat π
@@ -79,27 +85,27 @@ theorem all_next_congr (h : Equiv Φ Φ') : Equiv (⬝∀⬝◯Φ) (⬝∀⬝◯
   done
 
 @[simp]
-theorem all_untl_congr (h₁ : Equiv Φ Φ') (h₂ : Equiv Ψ Ψ') : Equiv (⬝∀(Φ ⬝U Ψ)) (⬝∀(Φ' ⬝U Ψ')) := by
-  simp [Equiv, satStateSet, SatState, StateSat, PathSat, Set.ext_iff] at *
+theorem all_untl_congr (h₁ : Equiv (p := p) Φ Φ') (h₂ : Equiv (p := p) Ψ Ψ') : Equiv (p := p) (⬝∀(Φ ⬝U Ψ)) (⬝∀(Φ' ⬝U Ψ')) := by
+  simp [Equiv, setOfSatStates, SatState, StateSatisfiable.StateSat, Set.ext_iff] at *
   intros _ _ _ _
   constructor
   . rintro sat π; obtain ⟨j, ⟨satJ, satK⟩⟩ := sat π; exact ⟨j, ⟨(h₂ _).1 satJ, fun k => (h₁ _).1 (satK k)⟩⟩
   . rintro sat π; obtain ⟨j, ⟨satJ, satK⟩⟩ := sat π; exact ⟨j, ⟨(h₂ _).2 satJ, fun k => (h₁ _).2 (satK k)⟩⟩
 
-theorem all_next_duality : Equiv (⬝∀⬝◯Φ) (⬝¬(⬝∃⬝◯⬝¬Φ)) := by
-  simp [Equiv, satStateSet, SatState, StateSat, PathSat]
+theorem all_next_duality : Equiv (p := p) (⬝∀⬝◯Φ) (⬝¬(⬝∃⬝◯⬝¬Φ)) := by
+  simp [Equiv, setOfSatStates, SatState, StateSatisfiable.StateSat, Set.ext_iff] at *
 
-theorem inevitable_duality : Equiv (⬝∀♢Φ) (⬝¬(⬝∃■⬝¬Φ)) := by
-  simp [Equiv, satStateSet, SatState, StateSat, PathSat, StateFormula.inevitable, PathFormula.untl]
+theorem inevitable_duality : Equiv (p := p) (⬝∀♢Φ) (⬝¬(⬝∃■⬝¬Φ)) := by
+  simp [Equiv, setOfSatStates, SatState, StateSatisfiable.StateSat, StateFormula.inevitable, PathFormula.untl]
 
-theorem exist_next_duality : Equiv (⬝∃⬝◯Φ) (⬝¬(⬝∀⬝◯⬝¬Φ)) := by
-  simp [Equiv, satStateSet, SatState, StateSat, PathSat]
+theorem exist_next_duality : Equiv (p := p) (⬝∃⬝◯Φ) (⬝¬(⬝∀⬝◯⬝¬Φ)) := by
+  simp [Equiv, setOfSatStates, SatState, StateSatisfiable.StateSat]
 
-theorem potential_duality : Equiv (⬝∃♢Φ) (⬝¬(⬝∀■⬝¬Φ)) := by
-  simp [Equiv, satStateSet, SatState, StateSat, PathSat, StateFormula.potential, PathFormula.untl]
+theorem potential_duality : Equiv (p := p) (⬝∃♢Φ) (⬝¬(⬝∀■⬝¬Φ)) := by
+  simp [Equiv, setOfSatStates, SatState, StateSatisfiable.StateSat, StateFormula.potential, PathFormula.untl]
 
-theorem all_untl_duality : Equiv (⬝∀(Φ ⬝U Ψ)) (⬝¬(⬝∃(⬝¬Ψ ⬝U (⬝¬Φ ⬝∧ ⬝¬Ψ))) ⬝∧ ⬝¬(⬝∃■⬝¬Ψ)) := by
-  simp [Equiv, satStateSet, SatState, StateSat, PathSat, Set.ext_iff] at *
+theorem all_untl_duality : Equiv (p := p) (⬝∀(Φ ⬝U Ψ)) (⬝¬(⬝∃(⬝¬Ψ ⬝U (⬝¬Φ ⬝∧ ⬝¬Ψ))) ⬝∧ ⬝¬(⬝∃■⬝¬Ψ)) := by
+  simp [Equiv, setOfSatStates, SatState, StateSatisfiable.StateSat, Set.ext_iff] at *
   intros _ _ _ _
   constructor
   . rintro sat
@@ -114,12 +120,13 @@ theorem all_untl_duality : Equiv (⬝∀(Φ ⬝U Ψ)) (⬝¬(⬝∃(⬝¬Ψ ⬝U
     obtain ⟨j, satΨ'⟩ := satΨ π
     exact ⟨j, ⟨satΨ', fun k => sorry⟩⟩
 
-theorem all_untl_expansion : Equiv (⬝∀(Φ ⬝U Ψ)) (Ψ ⬝∨ (Φ ⬝∧ (⬝∀⬝◯⬝∀(Φ ⬝U Ψ)))) := by
+theorem all_untl_expansion : Equiv (p := p) (⬝∀(Φ ⬝U Ψ)) (Ψ ⬝∨ (Φ ⬝∧ (⬝∀⬝◯⬝∀(Φ ⬝U Ψ)))) := by
   -- simp [Equiv, satStateSet, SatState, StateSat, PathSat, StateFormula.disj]
   -- intro s a ts
   -- ext x
   -- done
   sorry
+end StateFormula
 end Equiv
 
 end CTL
