CTL/Satisfaction.lean
@@ -6,58 +6,79 @@ import TS.EFin
 namespace CTL
 open TS
 
-variable {s a p : Type}
-         (ts : @TS s a p)
-         (Φ Φ₁ Φ₂ : @StateFormula p)
-         (φ φ₁ φ₂ : @PathFormula p)
+class StateSatisfiable (p α : Type) where
+  StateSat : {s a : Type}
+           → (ts : @TS s a p)
+           → (st : s)
+           → (Φ : α)
+           → Prop
 
-mutual
-  -- s ⊨ Φ
-  def StateSat :=
-    fun Φ st => match Φ with
-      | StateFormula.top => True
-      | ⬝a               => a ∈ ts.label st
-      | ⬝¬Φ              => ¬(StateSat Φ st)
-      | Φ₁ ⬝∧ Φ₂         => (StateSat Φ₁ st) ∧ (StateSat Φ₂ st)
-      | ⬝∃ φ             => ∃ π : PathFragment.From ts st, PathSat π.1.2 φ
-      | ⬝∀ φ             => ∀ π : PathFragment.From ts st, PathSat π.1.2 φ
-
-  -- π ⊨ φ
-  def PathSat (π : ts.PathFragment n) :=
-    fun
-      | ⬝◯ Φ   => StateSat Φ (π.second)
-      | Φ ⬝U Ψ => ∃ j : EFin (Order.succ n), (StateSat Ψ (π.get j)) ∧ ∀ k : EFin j.val, StateSat Φ (π.get (EFin.castLT j.lt k))
-end
+variable {p α β : Type}
+         [αSat : StateSatisfiable p α]
+         [βSat : StateSatisfiable p β]
+         {Φ : α}
+         {Ψ : β}
 
 -- Sat(Φ)
-def SatState := { st : s // StateSat ts Φ st }
-def satStateSet := @Set.range s (SatState ts Φ) Subtype.val
+def SatState {s a : Type} (ts : @TS s a p) (Φ : α) : Type :=
+  { st : s // StateSatisfiable.StateSat ts st Φ }
+def setOfSatStates {s a : Type} (ts : @TS s a p) (Φ : α) :=
+  @Set.range s (SatState ts Φ) Subtype.val
 
 -- TS ⊨ Φ
-def Sat := ∀ st ∈ ts.initial, StateSat ts Φ st
+def Sat {s a : Type} (ts: @TS s a p) (Φ : α) :=
+  ∀ st ∈ ts.initial, StateSatisfiable.StateSat ts st Φ
 
 @[simp]
-theorem Sat_iff_subset : (Sat ts Φ) ↔ (ts.initial ⊆ satStateSet ts Φ) :=
+theorem Sat_iff_initial_subset {s a : Type} (ts : @TS s a p) (Φ : α)
+  : (Sat ts Φ) ↔ (ts.initial ⊆ setOfSatStates ts Φ) :=
   by
     apply Iff.intro
     . intro sat st mem
       exact Set.mem_range_self (⟨st, sat st mem⟩ : SatState ts Φ)
     . intro sub st mem
       specialize sub mem
-      unfold satStateSet at sub
+      unfold setOfSatStates at sub
       rw [Set.mem_range] at sub
       obtain ⟨stSat, refl⟩ := sub
       rw [← refl]
       exact Subtype.property stSat
 
-namespace StateSat
-  @[simp]
-  theorem potentialAll_def {st : s} : StateSat ts (⬝∃■Φ) st ↔ ∃π : PathFragment.From ts st, ∀j, StateSat ts Φ (π.1.2.get j) := by
-    simp [StateFormula.potentialAll, StateSat, StateFormula.inevitable, PathSat]
 
-  @[simp]
-  theorem invariant_def : StateSat ts (⬝∀■Φ) st ↔ ∀π : PathFragment.From ts st, ∀j, StateSat ts Φ (π.1.2.get j) := by
-    simp [StateFormula.invariant, StateSat, StateFormula.potential, PathSat]
-end StateSat
+namespace StateFormula
+variable (Φ Φ₁ Φ₂ : @StateFormula p)
+         (φ φ₁ φ₂ : @PathFormula p)
 
+mutual
+  -- s ⊨ Φ
+  @[simp]
+  def StateSat (ts : @TS s a p) (st : s) :=
+    fun
+      | StateFormula.top => True
+      | ⬝a               => a ∈ ts.label st
+      | ⬝¬Φ              => ¬(StateSat ts st Φ)
+      | Φ₁ ⬝∧ Φ₂         => (StateSat ts st Φ₁) ∧ (StateSat ts st Φ₂)
+      | ⬝∃ φ             => ∃ π : PathFragment.From ts st, PathSat ts π.1.2 φ
+      | ⬝∀ φ             => ∀ π : PathFragment.From ts st, PathSat ts π.1.2 φ
+
+  -- π ⊨ φ
+  @[simp]
+  def PathSat (ts : @TS s a p) (π : ts.PathFragment n) :=
+    fun
+      | ⬝◯ Φ   => StateSat ts (π.second) Φ
+      | Φ ⬝U Ψ => ∃ j : EFin (Order.succ n), (StateSat ts (π.get j) Ψ) ∧ ∀ k : EFin j.val, StateSat ts (π.get (EFin.castLT j.lt k)) Φ
+end
+
+instance : StateSatisfiable p (@StateFormula p) where
+  StateSat := StateSat
+
+@[simp]
+theorem StateSat_potentialAll {st : s} : StateSat ts st (⬝∃■Φ) ↔ ∃π : PathFragment.From ts st, ∀j, StateSat ts (π.1.2.get j) Φ := by
+  simp
+
+@[simp]
+theorem StateStat_invariant : StateSat ts st (⬝∀■Φ) ↔ ∀π : PathFragment.From ts st, ∀j, StateSat ts (π.1.2.get j) Φ := by
+  simp
+
+end StateFormula
 end CTL
