CTL/Checking.lean
@@ -4,47 +4,46 @@ import TS.Basic
 import TS.Path
 
 namespace CTL
-variable {Φ Φ₁ Φ₂ : @StateFormula.ENF p}
+open StateFormula
 
-theorem top_satStateSet_def : satStateSet ts ⬝⊤ = Set.univ := by
-  simp [Set.ext_iff, satStateSet, SatState, StateSat]
+-- theorem top_satStateSet_def : setOfSatStates ts ⬝⊤ = Set.univ := by
+  -- simp [Set.ext_iff, setOfSatStates, SatState, StateSat]
 
-theorem prop_satStateSet_def : (satStateSet ts (⬝a) : Set s) = { st : s | a ∈ ts.label st } := by
-  simp [Set.ext_iff, satStateSet, SatState, StateSat]
+-- theorem prop_satStateSet_def : (setOfSatStates ts (⬝a) : Set s) = { st : s | a ∈ ts.label st } := by
+  -- simp [Set.ext_iff, setOfSatStates, SatState, StateSat]
 
-theorem conj_satStateSet_def : satStateSet ts (Φ₁.1 ⬝∧ Φ₂.1) = satStateSet ts Φ₁.1 ∩ satStateSet ts Φ₂.1 := by
-  simp [Set.ext_iff, satStateSet, SatState, StateSat]
+-- theorem conj_satStateSet_def : setOfSatStates ts (Φ₁.1 ⬝∧ Φ₂.1setOfSatStateseSet ts ΦsetOfSatStatesateSet ts Φ₂.1 := by
+  -- simp [Set.ext_iff, setOfSatStates, SatState, StateSat]
 
-theorem neg_satStateSet_def : satStateSet ts (⬝¬Φ.1) = Set.univ \ satStateSet ts Φ.1 := by
-  simp [Set.ext_iff, satStateSet, SatState, StateSat]
+-- theorem neg_satStateSet_def : setOfSatStates ts (⬝¬Φ.1) = Set.univ setOfSatStateset ts Φ.1 := by
+  -- simp [Set.ext_iff, setOfSatStates, SatState, StateSat]
 
-theorem exist_next_satStateSet_def : (satStateSet ts (⬝∃⬝◯Φ.1) : Set s) = { st : s | ts.post st ∩ (satStateSet ts Φ.1) ≠ ∅ } := by
-  simp [Set.ext_iff, satStateSet, SatState, StateSat]
-  intros st
-  constructor
-  . rintro ⟨⟨⟨_, π⟩, ⟨stIsHead, _⟩⟩, sat⟩
-    simp [PathSat] at sat
-    rw [← stIsHead]
-    exact ⟨π.second, ⟨π.second_mem_post_first, sat⟩⟩
-  . rintro ⟨st', ⟨memPost, sat⟩⟩
-    simp [PathSat]
-    exact ⟨_ , _⟩
+-- theorem exist_next_satStatsetOfSatStates(satStateSet ts (⬝∃⬝◯Φ.setOfSatStates = { st : s | ts.post st ∩ (satStateSet ts Φ.1) ≠ ∅ } := by
+  -- simp [Set.ext_iff, satStateSet, SatState, StateSat]
+  -- intros st
+  -- constructor
+  -- . rintro ⟨⟨⟨_, π⟩, ⟨stIsHead, _⟩⟩, sat⟩
+    -- simp [PathSat] at satsetOfSatStates
+    -- rw [← stIsHead]
+    -- exact ⟨π.second, ⟨π.second_mem_post_first, sat⟩⟩
+  -- . rintro ⟨st', ⟨memPost, sat⟩⟩
+    -- simp [PathSat]
+    -- exact ⟨_ , _⟩
 
-def computeSat (ts : @TS s a p) (Φ : @StateFormula.ENF p) : Set s :=
-  match Φ.1, Φ.2 with
-  | ⬝⊤, _ => Set.univ
-  | ⬝a, _ => { st : s | a ∈ ts.label st }
-  | Φ₁ ⬝∧ Φ₂, a => computeSat ts ⟨Φ₁, Φ.2⟩ ∩ satStateSet ts Φ₂
-  | ⬝∃⬝◯Φ => { st : s | ts.post st ∩ (satStateSet ts Φ) ≠ ∅ }
-  | ⬝∃(Φ ⬝U Ψ) => _
-  | ⬝¬(⬝∀(⬝⊤ ⬝U ⬝¬Φ)) => _
-  | ⬝¬Φ => Set.univ \ satStateSet ts Φ
-  | ⬝∀φ => _
+def computeSatENF (ts : @TS s a p) (Φ : @StateFormula.ENF p) : Set s :=
+  match Φ with
+  | ENF.top => Set.univ
+  | ENF.prop a => { st : s | a ∈ ts.label st }
+  | ENF.conj Φ₁ Φ₂ => (computeSatENF ts Φ₁) ∩ (computeSatENF ts Φ₂)
+  | ENF.neg Φ => Set.univ \ (computeSatENF ts Φ)
+  | ENF.existNext Φ => { st : s | ts.post st ∩ (computeSatENF ts Φ) ≠ ∅ }
+  | ENF.existUntil Φ Ψ => _
+  | ENF.potentialAll Φ => _
 
-theorem computerSat_def : computeSat ts Φ = satStateSet ts Φ :=
-  sorry
+-- theorem computerSat_def : computeSat ts Φ = satStateSet ts Φ :=
+  -- sorry
 
-instance : (ts : @TS s a p) → (Φ : @StateFormula p) → Decidable (Sat ts Φ) :=
-  fun ts Φ => _
+-- instance : (ts : @TS s a p) → (Φ : @StateFormula p) → Decidable (Sat ts Φ) :=
+  -- fun ts Φ => _
 
 end CTL
